\documentclass[a4paper,11pt,fleqn]{article}
\usepackage[utf8]{inputenc}
\usepackage{natbib}
\usepackage{graphicx}
\usepackage{amsmath}
\usepackage{geometry}
\geometry{left=2.0cm, right=2.0cm, top=4.0cm, bottom=2.0cm}

\title{Home work assignment in Mathematics }

\begin{document}
\maketitle
\large  Course: B1 Probability Theory and Statistical Inference, Fall 2016 
\vskip 1.0cm
Name: Jiayue Zeng
\vskip 1.0cm
Responsible teacher: Patrik Andersson 




\newpage
\textbf{Task 1}
\vskip 0.5cm
Find the derivative with respect to x of the following functions, simplify the result as much as possible.

\vskip 0.5cm
$ \left( a \right) \ f \left( x \right) = \frac{lnx}{x}$ 
\vskip 0.5cm
\qquad $ f' \left( x \right) =\frac{\left(lnx\right)'x-lnx}{x^2}= \frac{\frac{1}{x} x-lnx}{x^2} =\frac{1-lnx}{x^2}  $ 

\vskip 0.5cm
$\left( b \right) \ g \left( x \right) = e^{2\sqrt x}  $
\vskip 0.5cm
\qquad $ g' \left( x \right) = e^{2\sqrt x} \left(2\sqrt x \right)'=x^{-\frac{1}{2}}e^{2\sqrt x}  $

\vskip 0.5cm
$\left( c \right) \ h \left( x \right) = xe^{x^2} $
\vskip 0.5cm
\qquad $ h' \left( x \right) = \left(x\right)'e^{x^2}+x\left(e^{x^2}\right)'=e^{x^2}+2x^2e^{x^2}  $

\vskip 0.7cm



\textbf{Task 2}
\vskip 0.5cm
Find the derivative of the following functions with respect to x. Use the notation you find appropriate and motivate the steps. Simplify the result as much as possible.

\vskip 0.5cm
$ \left( a \right) \ f \left( x \right) = \frac{x+x^2}{3x^2}$ 
\vskip 0.5cm
\qquad $ f' \left( x \right) =\frac{\left(x+x^2\right)'\left(3x^2\right)-\left(3x^2\right)'\left(x+x^2\right)}{3x^2}=\frac{\left(1+2x\right)(3x^2)-(x+x^2)(6x)}{9x^4} $
\vskip 0.5cm
\qquad \qquad \;   $=\frac{3x^2+6x^3-6x^2-6x^3}{9x^4}=\frac{-3x^2}{9x^4}=-\frac{1}{3x^2}   $ 

\vskip 0.5cm
$\left( b \right) \ g \left( x \right) = exp(3x^3+1)  $
\vskip 0.5cm
\qquad $ g' \left( x \right) = exp(3x^3+1)(3x^3+1)' = 9x^2exp(3x^3 +1)  $



\newpage

\textbf{Task 3}
\vskip 0.5cm
Calculate the following integrals. The final answer should be exact. 
\vskip 0.5cm

$\left( a \right) \, \int_{0}^{1} e^{-3x}dx = [-\frac{1}{3}e^{-3x}]_0^1 = (-\frac{1}{3} e^{-3})-(-\frac{1}{3}e^0) = \frac{1}{3}-\frac{1}{3}e^{-3}  $
\vskip 0.5cm

$\left( b \right) \, \int_{1}^{2}\frac{1}{\sqrt{2x}}dx = [\sqrt{2x}]_{1}^{2} = \sqrt{4}-\sqrt{2}=2-\sqrt 2
$
\vskip 0.5cm

$\left( c \right) \,  \int_{1}^{2}\frac{2x^2+x+3}{x}dx = \int_{1}^{2}2x+1+\frac{3}{x}dx = [x^2+x+3lnx]_{1}^{2}  $
\vskip 0.5cm
\qquad \; $= (4+2+3ln2)-(1+1-3ln1) = 4+3ln2  $
\vskip 0.7cm


\textbf{Task 4}
\vskip 0.5cm
Calculate the following integrals, simplify the result as much as possible. 
\vskip 0.5cm
$\left( a \right)$  Consider the function $\;  u(x)=x^2 $, we have $\; 
u(x)'=2x $.
\vskip 0.5cm
$\int xe^{x^2}dx = \int (xe^{u}) (\frac{1}{2x})du= \int \frac{1}{2}e^u du = \frac{1}{2}e^{u}+ C = \frac{1}{2}e^{x^2}+C  $
\vskip 0.5cm

$\left( b \right)\, $ 
Choose $\; f(x)=log(x), g'(x)=x $ which gives $\; f'(x)=\frac{1}{x}\; $and $\; g(x)=\frac{1}{2}x^2$. 
\vskip 0.5cm
$  \int xlog(x)dx = f(x)g(x)- \int f'(x)g(x)dx $
\vskip 0.5cm
\qquad \qquad \quad $ =\frac{1}{2}x^2 log(x)-\int \frac{1}{2}x^2\frac{1}{x}dx $
\vskip 0.5cm
\qquad \qquad \quad $ =\frac{1}{2}x^2 log(x)-\frac{1}{4}x^2+C $

\vskip 0.7cm
\textbf{Task 5}
\vskip 0.5cm
\quad a) Find the value of c that makes p(x) a probability density function.
\vskip 0.5cm
If p(x) is a probability function, we must ensure that:
$\;F(\infty)=\int_{-\infty}^{\infty} p(x)dx =1 $. 
And we know that, $\;F(\infty)=\int_{-\infty}^{\infty} p(x)dx = \int_{1}^{2} p(x)dx $
\vskip 0.5cm
\large $\int_{1}^{2}\frac{c}{x}dx = c\int_{1}^{2} \frac{1}{x}dx 
= c[ln(x)]_{1}^{2}$
\vskip 0.5cm
\qquad \quad $\, =c(ln2-0)=cln2=1 $
\vskip 0.5cm
So, \quad
\large $\; c=\frac{1}{ln2} $

\newpage
\vskip 0.5cm
b) Find the expected value 
\vskip 0.5cm
$\mu_{X} = E(X) = \int_{1}^{2} xp(x)dx 
= \int_{1}^{2}x\frac{1}{ln2}\frac{1}{x} dx $
\vskip 0.5cm
\quad $ \; \, = \int_{1}^{2} \frac{1}{ln2}dx
= \frac{1}{ln2}[x]_{1}^{2}  
= \frac{1}{ln2}$


\vskip 0.5cm
c) Find the variance
\vskip 0.5cm
$ V(X)=E(X^2)-\mu_{X}^{2}

\vskip 0.5cm
$
E(X^2)=\int_{1}^{2}x^{2}p(x)dx
= \int_{1}^{2}x^{2}\frac{1}{ln2}\frac{1}{x}dx
= \frac{1}{ln2}\int_{1}^{2}xdx
= \frac{1}{ln2}[\frac{1}{2}x^2]_{1}^{2}
= \frac{1}{ln2}(2-\frac{1}{2})
= \frac{3}{2ln2}
$
\vskip 0.5cm
$
V(X) =E(X^2)-\mu_{X}^{2} = \frac{3}{2ln2}-(\frac{1}{ln2})^2
$


\end{document}
